theories/typing/int.v
@@ -21,7 +21,7 @@ Section int.
 
   Lemma type_int_instr z : typed_val #z int (λ post, post z).
   Proof.
-    iIntros (?????) "_ _ _ $$ _ Obs". iMod persistent_time_receipt_0 as "Time".
+    iIntros (?????) "_ _ _ _ $$ _ Obs". iMod persistent_time_receipt_0 as "Time".
     iApply wp_value. iExists -[const z]. iFrame "Obs". iSplit; [|done].
     rewrite tctx_hasty_val'; [|done]. iExists 0%nat. iFrame "Time". by iExists z.
   Qed.
@@ -36,7 +36,7 @@ Section int.
     ⊢ typed_instr_ty E L +[p1 ◁ int; p2 ◁ int] (p1 + p2) int
       (λ post '(-[z; z']), post (z + z')).
   Proof.
-    iIntros (??(?&?&[])) "_ _ _ $$ (P1 & P2 &_) Obs".
+    iIntros (??(?&?&[])) "_ _ _ _ $$ (P1 & P2 &_) Obs".
     wp_apply (wp_hasty with "P1"). iIntros (? d _) "Time". iIntros ((z&->&[=->])).
     wp_apply (wp_hasty with "P2"). iIntros (?? _) "_". iIntros ((z'&->&[=->])).
     wp_op. iExists -[const (z + z')]. iFrame "Obs". rewrite right_id
@@ -57,7 +57,7 @@ Section int.
     ⊢ typed_instr_ty E L +[p1 ◁ int; p2 ◁ int] (p1 - p2) int
       (λ post '(-[z; z']), post (z - z')).
   Proof.
-    iIntros (??(?&?&[])) "_ _ _ $$ (P1 & P2 &_) Obs".
+    iIntros (??(?&?&[])) "_ _ _ _ $$ (P1 & P2 &_) Obs".
     wp_apply (wp_hasty with "P1"). iIntros (? d _) "Time". iIntros ((z&->&[=->])).
     wp_apply (wp_hasty with "P2"). iIntros (?? _) "_". iIntros ((z'&->&[=->])).
     wp_op. iExists -[const (z - z')]. iFrame "Obs". rewrite right_id
@@ -78,7 +78,7 @@ Section int.
     ⊢ typed_instr_ty E L +[p1 ◁ int; p2 ◁ int] (p1 ≤ p2) bool_ty
       (λ post '(-[z; z']), post (bool_decide (z ≤ z'))).
   Proof.
-    iIntros (??(?&?&[])) "_ _ _ $$ (P1 & P2 &_) Obs".
+    iIntros (??(?&?&[])) "_ _ _ _ $$ (P1 & P2 &_) Obs".
     wp_apply (wp_hasty with "P1"). iIntros (? d _) "Time". iIntros ((z&->&[=->])).
     wp_apply (wp_hasty with "P2"). iIntros (?? _) "_". iIntros ((z'&->&[=->])).
     wp_op. iExists -[const (bool_decide (z <= z'))]. iFrame "Obs".
